src/Fresh_Start.thy
@@ -1,0 +1,231 @@
+theory
+  Fresh_Start
+imports
+  Main
+  "~~/src/HOL/Library/Monad_Syntax"
+begin
+
+type_synonym ('id, 'v) elt = "'id \<times> 'v"
+
+fun insert :: "('id::{linorder}, 'v) elt list \<Rightarrow> ('id, 'v) elt \<Rightarrow> 'id option \<rightharpoonup> ('id::{linorder}, 'v) elt list" where
+  "insert [] e     None     = Some [e]" |
+  "insert [] e     (Some i) = None" |
+  "insert (x#xs) e None     =
+     (if fst x < fst e then
+        Some (e#x#xs)
+      else
+        case insert xs e None of
+          None   \<Rightarrow> None
+        | Some t \<Rightarrow> Some (x#t))" |
+  "insert (x#xs) e (Some i) =
+     (if fst x = i then
+        case insert xs e None of
+          None   \<Rightarrow> None
+        | Some t \<Rightarrow> Some (x#t)
+      else
+        case insert xs e (Some i) of
+          None   \<Rightarrow> None
+        | Some t \<Rightarrow> Some (x#t))"
+
+lemma insert_None_condition1 [elim!, dest]:
+  assumes "insert xs e (Some i) = None"
+  shows   "xs = [] \<or> i \<notin> set (map fst xs)"
+sorry
+
+lemma insert_None_condition2 [elim!, dest]:
+  assumes "insert xs e None = None"
+  shows   "False"
+using assms
+  by (induction xs, auto, case_tac "a < fst e"; clarsimp) (case_tac "Fresh_Start.insert xsa e None"; clarsimp)
+
+lemma insert_Some_condition1 [elim!, dest]:
+  assumes "insert xs e None = Some []"
+  shows   "False"
+using assms
+  by (induction xs, auto, case_tac "a < fst e"; clarsimp) (case_tac "Fresh_Start.insert xsa e None"; clarsimp)
+
+lemma insert_commutes:
+  assumes "distinct (map fst (e1#e2#xs))" "the i1 \<noteq> fst e2" "the i2 \<noteq> fst e1"
+  shows   "insert xs e1 i1 \<bind> (\<lambda>ys. insert ys e2 i2) = insert xs e2 i2 \<bind> (\<lambda>ys. insert ys e1 i1)"
+using assms
+  apply(induction xs)
+  (* Empty case *)
+  apply clarsimp
+  apply(cases i1; clarsimp; cases i2; clarsimp)
+  apply force
+  (* Step case *)
+  apply(cases i1; clarsimp; cases i2; clarsimp)
+  apply(case_tac "a < fst e1 \<and> fst e1 < fst e2"; clarsimp)
+    apply(case_tac "Fresh_Start.insert xs e1 None"; clarsimp)
+    apply(case_tac "Fresh_Start.insert xs e2 None"; clarsimp)
+    apply(drule insert_None_condition2, simp)+
+    apply(case_tac "Fresh_Start.insert xs e2 None"; clarsimp)
+    apply(drule insert_None_condition2, simp)
+    apply force
+    apply(case_tac "Fresh_Start.insert xs e1 None"; clarsimp)
+    apply(drule insert_None_condition2, simp)
+    apply(case_tac "Fresh_Start.insert xs e2 None"; clarsimp)
+    apply(drule insert_None_condition2, simp)
+    apply auto[1]
+  apply(case_tac "a < fst e2 \<and> fst e2 < fst e1"; clarsimp)
+    apply(case_tac "Fresh_Start.insert xs e1 None"; clarsimp)
+    apply(drule insert_None_condition2, simp)
+    apply(case_tac "Fresh_Start.insert xs e2 (Some aa)"; clarsimp)
+    apply(case_tac "Fresh_Start.insert xs e2 None"; clarsimp)
+    apply(drule insert_None_condition2, simp)
+    apply(case_tac "Fresh_Start.insert xs e1 None"; clarsimp)
+    apply force
+    apply(case_tac "Fresh_Start.insert xs e2 None"; clarsimp)
+    apply(drule insert_None_condition2, simp)
+    apply(case_tac "Fresh_Start.insert ab e2 None"; clarsimp)
+    apply(drule insert_None_condition2, simp)
+    apply(case_tac "Fresh_Start.insert a e1 None"; clarsimp)
+    apply auto[1]
+    
+  apply(case_tac "a < fst e1 \<and> a > fst e2"; clarsimp)
+    apply(case_tac "Fresh_Start.insert xs e2 None"; clarsimp)
+    apply(case_tac "Fresh_Start.insert xs e1 None"; clarsimp)
+    apply(drule insert_None_condition2, simp)
+    apply(case_tac "Fresh_Start.insert xs e2 None"; clarsimp)
+    apply(case_tac "Fresh_Start.insert xs e2 None"; clarsimp)
+    apply(drule insert_None_condition2, simp)
+    apply(case_tac "Fresh_Start.insert xs e1 None"; clarsimp)
+    apply auto[1]
+  apply(case_tac "a < fst e2 \<and> a > fst e1"; clarsimp)
+    apply(case_tac "Fresh_Start.insert xs e1 None"; clarsimp)
+    apply(case_tac "Fresh_Start.insert xs e2 None"; clarsimp)
+    apply(drule insert_None_condition2, simp)
+    apply(case_tac "Fresh_Start.insert xs e1 None"; clarsimp)
+    apply(case_tac "Fresh_Start.insert xs e1 None"; clarsimp)
+    apply(drule insert_None_condition2, simp)
+    apply(case_tac "Fresh_Start.insert xs e2 None"; clarsimp)
+    apply auto[1]
+  apply(case_tac "fst e1 < fst e2 \<and> fst e2 < a"; clarsimp)
+    apply(case_tac "Fresh_Start.insert xs e1 None"; clarsimp)
+    apply(drule insert_None_condition2, simp)
+    apply(case_tac "Fresh_Start.insert xs e2 None"; clarsimp)
+    apply(case_tac "Fresh_Start.insert xs e2 None"; clarsimp)
+    apply(drule insert_None_condition2, simp)
+    apply(case_tac "Fresh_Start.insert xs e1 None"; clarsimp)
+    apply(drule insert_None_condition2, simp)
+    apply auto[1]
+  apply(case_tac "fst e2 < fst e1 \<and> fst e1 < a"; clarsimp)
+    apply(case_tac "Fresh_Start.insert xs e1 None"; clarsimp)
+    apply(drule insert_None_condition2, simp)
+    apply(case_tac "Fresh_Start.insert xs e2 None"; clarsimp)
+    apply(drule insert_None_condition2, simp)
+    apply(case_tac "Fresh_Start.insert xs e2 (Some aa)"; clarsimp)
+    apply(case_tac "Fresh_Start.insert ab e2 None"; clarsimp)
+    apply(drule insert_None_condition2, simp)
+    apply(case_tac "Fresh_Start.insert ac e1 None"; clarsimp)
+    
+    
+
+
+(*
+  apply(induction rule: insert.induct)
+    (* First case *)
+    apply(cases "i1"; simp; cases "i2"; simp; (force+))
+    (* Second case *)
+    apply(cases "i1"; simp; cases "i2"; simp; (force+))
+    (* Third case *)
+    apply(case_tac "fst x < fst e")
+      (* If: true case *)
+      apply clarsimp
+      apply(case_tac "Fresh_Start.insert ((a, b) # xs) e2 i2"; clarsimp)
+      apply(case_tac "i2"; clarsimp)
+      apply(case_tac "a < fst e2"; clarsimp)
+      apply(case_tac "Fresh_Start.insert xs e2 None"; clarsimp)
+      apply(case_tac "i2"; clarsimp)
+      apply(case_tac "a < fst e2"; clarsimp)
+      apply force
+      apply(case_tac "Fresh_Start.insert xs e2 None"; clarsimp)
+      apply simp
+      apply(case_tac "a = ac"; clarsimp)
+      apply(case_tac "Fresh_Start.insert xs e2 None"; clarsimp)
+      apply(case_tac "Fresh_Start.insert xs e2 (Some ac)"; clarsimp)
+      (* If: false case *)
+      apply clarsimp
+      apply(case_tac "Fresh_Start.insert xs (aa, ba) None"; clarsimp)
+      apply(drule insert_None_condition2, force)
+      apply(cases "i2"; clarsimp)
+      apply(case_tac "Fresh_Start.insert xs e2 None"; clarsimp)
+      apply(drule insert_None_condition2, force)
+      apply force
+      apply(case_tac "a = ac"; clarsimp)
+      apply(case_tac "Fresh_Start.insert xs e2 None"; clarsimp)
+      apply(case_tac "Fresh_Start.insert xs e2 (Some ac)"; clarsimp)
+      apply(drule insert_None_condition2, force)
+      apply(drule insert_None_condition2, force)
+      apply(case_tac "Fresh_Start.insert ab e2 None"; clarsimp)
+      apply(case_tac "Fresh_Start.insert a (aa, ba) None"; clarsimp)
+      apply(case_tac "Fresh_Start.insert a (aa, ba) None"; clarsimp)
+      apply(case_tac "Fresh_Start.insert xs e2 (Some ac)"; clarsimp)
+      apply(drule insert_None_condition1, erule disjE)
+        apply(clarsimp)
+        apply(drule insert_Some_condition1, force)
+        apply(drule insert_None_condition1, erule disjE)
+          apply clarsimp
+          apply(case_tac "aa < fst e2"; clarsimp)
+          apply(case_tac "fst e2 < aa"; clarsimp)
+          apply simp
+          apply(case_tac "fst e2 < aa"; clarsimp)
+*)
+
+(*
+    apply(cases "i1"; simp; cases "i2"; simp; (force+))
+    apply(cases "i1"; simp; cases "i2"; simp)
+    apply(case_tac "fst x < fst e"; clarsimp)
+    apply(cases "i2"; simp)
+    apply(case_tac "fst e2 < aa"; clarsimp)
+    apply(case_tac "a < fst e2"; clarsimp)
+    apply force
+    apply(case_tac "Fresh_Start.insert xs e2 None"; clarsimp; force; force)
+    apply(case_tac "Fresh_Start.insert xs e2 None"; clarsimp; force; force)
+    apply(case_tac "a = ab"; clarsimp)
+    apply(case_tac "Fresh_Start.insert xs e2 None"; clarsimp)
+    apply(case_tac "Fresh_Start.insert xs e2 (Some ab)"; clarsimp)
+    apply(case_tac "Fresh_Start.insert xs (aa, ba) None"; clarsimp)
+    apply(cases i2; clarsimp)
+    apply(case_tac "fst e2 < aa"; clarsimp)
+    apply(case_tac "a < fst e2"; clarsimp)
+    apply(case_tac "Fresh_Start.insert xs e2 None"; clarsimp)
+    apply(case_tac "Fresh_Start.insert xs e2 None"; clarsimp)
+    apply(case_tac "a = ab"; clarsimp)
+    apply(case_tac "Fresh_Start.insert xs e2 None"; clarsimp)
+    apply(case_tac "Fresh_Start.insert a (aa, ba) None"; clarsimp)
+    apply(case_tac "Fresh_Start.insert xs e2 (Some ab)"; clarsimp)
+    apply(case_tac "Fresh_Start.insert xs e2 i2"; clarsimp)
+    apply(case_tac "Fresh_Start.insert ((a, b) # xs) e2 i2"; clarsimp)
+    apply(case_tac "i2"; clarsimp)
+    apply(case_tac "Fresh_Start.insert xs e2 None"; clarsimp)
+    apply(drule insert_None_condition1)
+    apply(erule disjE; clarsimp)
+    apply(case_tac "Fresh_Start.insert ab e2 None"; clarsimp)
+    apply(case_tac "i2"; clarsimp)
+    apply(case_tac "a < fst e2"; clarsimp)
+    apply(drule insert_None_condition2)
+    apply force
+    apply(case_tac "a = ad"; clarsimp)
+    apply(case_tac "Fresh_Start.insert xs e2 None"; clarsimp)
+    apply(case_tac "Fresh_Start.insert a (aa, ba) None"; clarsimp)
+    apply(case_tac "Fresh_Start.insert ab e2 None"; clarsimp)
+    apply(case_tac "Fresh_Start.insert ab e2 None"; clarsimp)
+    apply(drule insert_None_condition1)
+    apply(erule disjE; clarsimp)
+    apply(drule insert_Some_condition1, force)
+    apply(drule insert_None_condition1, erule disjE, clarsimp)
+*)    
+(*
+  apply(case_tac "Fresh_Start.insert xs e None"; clarsimp)
+  apply(case_tac "Fresh_Start.insert xs e2 None"; clarsimp; force; force)
+  apply(case_tac "Fresh_Start.insert xs e2 None"; clarsimp; force; force)
+  apply(case_tac "Fresh_Start.insert xs e2 None"; clarsimp)
+  apply(case_tac "Fresh_Start.insert xs e2 (Some ab)"; clarsimp)
+  apply(case_tac "Fresh_Start.insert xs (aa, ba) None"; clarsimp)
+  apply(case_tac "Fresh_Start.insert ac e2 None"; clarsimp)
+  *)
+  
+  
+
+end
